pure/Learn.Util.fst
@@ -20,9 +20,19 @@ module T = FStar.Tactics
 
 (* from F* tutorial *)
 let funext_on_eta (#a : Type) (#b: a -> Type) (f g : (x:a -> b x))
-                  (hp : (x:a -> Lemma (f x == g x)))
+                  (hp : (x:a -> squash (f x == g x)))
   : squash (eta f == eta g)
   = _ by T.(norm [delta_only [`%eta]];
+          pointwise (fun _ ->
+             try_with
+                     (fun _ -> mapply (quote hp))
+                     (fun _ -> trefl()));
+           trefl())
+
+let funext_on_eta_gtot (#a : Type) (#b: a -> Type) (f g : (x:a -> GTot (b x)))
+                  (hp : (x:a -> squash (f x == g x)))
+  : squash (eta_gtot f == eta_gtot g)
+  = _ by T.(norm [delta_only [`%eta_gtot]];
           pointwise (fun _ ->
              try_with
                      (fun _ -> mapply (quote hp))
